Consequences

hulls.v
@@ -5,17 +5,17 @@ Require Import MSetAVL.
 
 Module N2 := PairOrderedType Nat_as_OT Nat_as_OT.
 Module Triangle := PairOrderedType Nat_as_OT N2.
-Module TriangleSet := MSetAVL.Make Triangle.
+Module TS := MSetAVL.Make Triangle.
 
 Notation "[ x , y , z ]" := (x,(y,z)).
-Notation "{{ x , .. , y }}" := (TriangleSet.add x .. (TriangleSet.add y TriangleSet.empty) .. ).
-Notation "{{}}" := TriangleSet.empty.
+Notation "{{ x , .. , y }}" := (TS.add x .. (TS.add y TS.empty) .. ).
+Notation "{{}}" := TS.empty.
 
 Definition insert csq_orig t csq_new :=
-  if TriangleSet.mem t csq_orig then
+  if TS.mem t csq_orig then
     csq_new
   else
-    TriangleSet.add t csq_new.
+    TS.add t csq_new.
 
 Definition step1 csq_orig t csq_new :=
   match t with
@@ -27,7 +27,7 @@ Definition step4_aux csq_orig a b d t csq_new :=
   match t with
       [b',c,d'] =>
       if N2.eq_dec (b,d) (b',d') then
-        if TriangleSet.mem [c,a,d] csq_orig then
+        if TS.mem [c,a,d] csq_orig then
           insert csq_orig [a,b,c] csq_new
         else
           csq_new
@@ -38,14 +38,14 @@ Definition step4_aux csq_orig a b d t csq_new :=
 Definition step4 csq_orig t csq_new :=
   match t with
       [a,b,d] =>
-      TriangleSet.fold (step4_aux csq_orig a b d) csq_orig csq_new
+      TS.fold (step4_aux csq_orig a b d) csq_orig csq_new
   end.
 
 Definition step5_aux_aux csq_orig a b c d t csq_new :=
   match t with
       [a',b',e] =>
       if N2.eq_dec (a, b) (a' ,b') then
-        if TriangleSet.mem [a,c,d] csq_orig && TriangleSet.mem [a,d,e] csq_orig then
+        if TS.mem [a,c,d] csq_orig && TS.mem [a,d,e] csq_orig then
           insert csq_orig [a,c,e] csq_new
         else
           csq_new
@@ -57,7 +57,7 @@ Definition step5_aux csq_orig a b c t csq_new :=
   match t with
       [a',b',d] =>
       if N2.eq_dec (a, b) (a' ,b') then
-        TriangleSet.fold (step5_aux_aux csq_orig a b c d) csq_orig csq_new
+        TS.fold (step5_aux_aux csq_orig a b c d) csq_orig csq_new
       else
         csq_new
   end.
@@ -65,36 +65,66 @@ Definition step5_aux csq_orig a b c t csq_new :=
 Definition step5 csq_orig t csq_new :=
   match t with
       [a,b,d] =>
-      TriangleSet.fold (step5_aux csq_orig a b d) csq_orig csq_new
+      TS.fold (step5_aux csq_orig a b d) csq_orig csq_new
   end.
 
 (*** Tests step1, step4, step5  ***)
 Definition test1 := {{[1,2,3],[2,3,4]}}.
-Compute (TriangleSet.elements (step1 test1 [1,2,3] {{}})).
+Compute (TS.elements (step1 test1 [1,2,3] {{}})).
 
 Definition test1' := {{[1,2,3],[2,3,1]}}.
-Compute (TriangleSet.elements (step1 test1' [1,2,3] {{}})).
+Compute (TS.elements (step1 test1' [1,2,3] {{}})).
 
 Definition test4 := {{[1,2,3],[2,4,3],[4,1,3]}}.
-Compute (TriangleSet.elements (step4 test4 [1,2,3] {{}})).
+Compute (TS.elements (step4 test4 [1,2,3] {{}})).
 
 Definition test5 := {{[1,2,3],[1,2,4],[1,2,5],[1,3,4],[1,4,5]}}.
-Compute (TriangleSet.elements (step5 test5 [1,2,3] {{}})).
+Compute (TS.elements (step5 test5 [1,2,3] {{}})).
 
 Definition step145 csq_orig :=
-  let csq_new := TriangleSet.fold (step1 csq_orig) csq_orig TriangleSet.empty in
-  let csq_new' := TriangleSet.fold (step4 csq_orig) csq_orig csq_new in
-  let csq_new'' := TriangleSet.fold (step5 csq_orig) csq_orig csq_new' in
-  if TriangleSet.is_empty csq_new then
+  let csq_new := TS.fold (step1 csq_orig) csq_orig TS.empty in
+  let csq_new' := TS.fold (step4 csq_orig) csq_orig csq_new in
+  let csq_new'' := TS.fold (step5 csq_orig) csq_orig csq_new' in
+  if TS.is_empty csq_new then
     inl csq_orig
   else
-    inr (TriangleSet.union csq_orig csq_new).
+    inr (TS.union csq_orig csq_new).
+
+Definition csq_proj (r : TS.t + TS.t) := match r with
+                           | inl csq => csq
+                           | inr csq => csq
+                         end.
 
 Fixpoint sat145 csq fuel {struct fuel} :=
   match fuel with
     | O => csq
-    | S p => match step145 csq with
-               | inl csq' => csq'
-               | inr csq' => sat145 csq' p
-             end
+    | S p =>
+      match step145 csq with
+        | inl csq' => csq'
+        | inr csq' => sat145 csq' p
+      end
   end.
+
+Inductive Conseq : TS.t -> Triangle.t -> Prop :=
+  | Id : forall ts t, TS.In t ts -> Conseq ts t
+  | Rule1 : forall ts a b c, TS.In [a,b,c] ts -> Conseq ts [b,c,a]
+  | Rule4 : forall ts a b c d, TS.In [a,b,d] ts -> TS.In [b,c,d] ts -> TS.In [c,a,d] ts -> Conseq ts [a,b,c]
+  | Rule5 : forall ts a b c d e, TS.In [a,b,c] ts -> TS.In [a,b,d] ts -> TS.In [a,b,e] ts -> TS.In [a,c,d] ts -> TS.In [a,d,e] ts -> Conseq ts [a,c,e].
+
+Inductive Conseqs : TS.t -> TS.t -> Prop :=
+  | Conseq_add : forall ts ts', (forall t, (TS.In t ts') -> Conseq ts t) -> Conseqs ts ts'
+  | Conseq_trans : forall ts ts' ts'', Conseqs ts ts' -> Conseqs ts' ts'' -> Conseqs ts ts''.
+
+Lemma step145_correct : forall ts t, TS.In t (csq_proj (step145 ts)) -> Conseq ts t.
+Proof.
+
+Admitted.
+
+Theorem sat145_correct : forall ts fuel, Conseqs ts (sat145 ts fuel).
+Proof.
+
+Admitted.
+
+
+Definition inconsistent csq :=
+  TS.exists_ (fun t => match t with [a,b,c] => TS.mem [a,c,b] csq end).
